

Algebra - Solutions to Paul's Online Math Notes Assignment Problems

Justin Lin

1. Preliminaries

1.1. Integer Exponents

For problems 1 - 10, evaluate the given expression and write the answer as a single number with no exponents.

1. $2 \cdot 5^2 + (-4)^2$

$$\begin{aligned} 2 \cdot 5^2 + (-4)^2 &= 2 \cdot 25 + 16 \\ &= 50 + 16 \\ &= 66 \end{aligned}$$

2. $6^0 - 3^5$

$$\begin{aligned} 6^0 - 3^5 &= 1 - 243 \\ &= -242 \end{aligned}$$

3. $3 \cdot 4^3 + 2 \cdot 3^2$

$$\begin{aligned} 3 \cdot 4^3 + 2 \cdot 3^2 &= 3 \cdot 64 + 2 \cdot 9 \\ &= 192 + 18 \\ &= 210 \end{aligned}$$

4. $(-1)^4 + 2(-3)^4$

$$\begin{aligned} (-1)^4 + 2(-3)^4 &= 1 + 2(81) \\ &= 1 + 162 \\ &= 163 \end{aligned}$$

5. $7^0(4^2 \cdot 3^2)^2$

$$\begin{aligned} 7^0(4^2 \cdot 3^2)^2 &= 1(16 \cdot 9)^2 \\ &= (144)^2 \\ &= 20,736 \end{aligned}$$

6. $-4^3 + (-4)^3$

$$\begin{aligned} -4^3 + (-4)^3 &= -64 + (-64) \\ &= -64 - 64 \\ &= -128 \end{aligned}$$

7. $8 \cdot 2^{-3} + 16^0$

$$\begin{aligned}
 8 \cdot 2^{-3} + 16^0 &= 8 \cdot \frac{1}{8} + 1 \\
 &= 1 + 1 \\
 &= 2
 \end{aligned}$$

$$8. \ (2^{-1} + 3^{-1})^{-1}$$

$$\begin{aligned}
 (2^{-1} + 3^{-1})^{-1} &= \left(\frac{1}{2} + \frac{1}{3} \right)^{-1} \\
 &= \frac{1}{\frac{1}{2} + \frac{1}{3}} \\
 &= \frac{1}{\frac{3}{6} + \frac{2}{6}} \\
 &= \frac{1}{\frac{5}{6}} \\
 &= \frac{6}{5}
 \end{aligned}$$

$$9. \ \frac{3^2 \cdot (-2)^3}{6^{-2}}$$

$$\begin{aligned}
 \frac{3^2 \cdot (-2)^3}{6^{-2}} &= \frac{9 \cdot -8}{\frac{1}{36}} \\
 &= -72 \cdot 36 \\
 &= -2,592
 \end{aligned}$$

$$10. \ \frac{4^{-2} \cdot 5^3}{3^{-4}}$$

$$\begin{aligned}
 \frac{4^{-2} \cdot 5^3}{3^{-4}} &= \frac{\left(\frac{1}{16} \right) \cdot 125}{\frac{1}{81}} \\
 &= \left(\frac{125}{16} \right) \cdot 81 \\
 &= \frac{10125}{16}
 \end{aligned}$$

For problems 11 - 18, simplify the given expression and write the answer with only positive exponents.

11. $(3x^{-2}y^{-4})^{-1}$

$$\begin{aligned}(3x^{-2}y^{-4})^{-1} &= 3x^{-2 \cdot -1}y^{-4 \cdot -1} \\ &= 3x^2y^4\end{aligned}$$

12. $\left[(2a^2)^{-3}b^4\right]^{-3}$

$$\begin{aligned}\left[(2a^2)^{-3}b^4\right]^{-3} &= \left[2^{-3}a^{2 \cdot (-3)}b^4\right]^{-3} \\ &= 2^{-3 \cdot -3}a^{-6 \cdot -3}b^{4 \cdot -3} \\ &= 2^9a^{18}b^{-12} \\ &= \frac{512a^{18}}{b^{12}}\end{aligned}$$

13. $\frac{c^{-6}b^{10}}{b^9c^{-11}}$

$$\begin{aligned}\frac{c^{-6}b^{10}}{b^9c^{-11}} &= c^{(-6)-(-11)}b^{10-9} \\ &= c^{-6+11}b^1 \\ &= c^5b\end{aligned}$$

14. $\frac{4a^3(b^2a)^{-4}}{c^{-6}a^2b^{-7}}$

$$\begin{aligned}\frac{4a^3(b^2a)^{-4}}{c^{-6}a^2b^{-7}} &= \frac{4a^3b^{2 \cdot -4}a^{1 \cdot -4}}{c^{-6}a^2b^{-7}} \\ &= \frac{4a^{3-4}b^{-8}}{c^{-6}a^2b^{-7}} \\ &= \frac{4a^{-1-2}b^{-8-(-7)}}{c^{-6}} \\ &= \frac{4a^{-3}b^{-1}}{c^{-6}} \\ &= \frac{4c^6}{a^3b}\end{aligned}$$

15. $\frac{(6v^2)^{-1}w^{-4}}{(2v)^{-3}w^{10}}$

$$\begin{aligned}
\frac{(6v^2)^{-1}w^{-4}}{(2v)^{-3}w^{10}} &= \frac{6^{-1}v^{2(-1)}w^{-4}}{2^{-3}v^{-3}w^{10}} \\
&= \frac{\left(\frac{1}{6}\right)v^{-2}w^{-4}}{\left(\frac{1}{8}\right)v^{-3}w^{10}} \\
&= \left(\frac{8}{6}\right) \cdot v^{-2-(-3)}w^{-4-10} \\
&= \left(\frac{4}{3}\right) \cdot v^1 \cdot w^{-14} \\
&= \frac{4v}{3w^{14}}
\end{aligned}$$

$$16. \left[\frac{(8x^{21})^0 y^{-3} x^8}{y^{-9} x^{-1}} \right]^6$$

$$\begin{aligned}
\left[\frac{(8x^{21})^0 y^{-3} x^8}{y^{-9} x^{-1}} \right]^6 &= \left[\frac{8^0 x^{21 \cdot 0} y^{-3} x^8}{y^{-9} x^{-1}} \right]^6 \\
&= [1 \cdot y^{-3-(-9)} \cdot x^{8-(-1)}]^6 \\
&= (y^6 x^9)^6 \\
&= y^{6 \cdot 6} x^{9 \cdot 6} \\
&= y^{36} x^{54}
\end{aligned}$$

$$17. \left(\frac{a^2 b^{-4} c^{-1}}{b^{-9} c^8 a^{-4}} \right)^{-2}$$

$$\begin{aligned}
\left(\frac{a^2 b^{-4} c^{-1}}{b^{-9} c^8 a^{-4}} \right)^{-2} &= (a^{2-(-4)} b^{-4-(-9)} c^{-1-8})^{-2} \\
&= (a^6 b^5 c^{-9})^{-2} \\
&= a^{6(-2)} b^{5(-2)} c^{-9(-2)} \\
&= a^{-12} b^{-10} c^{18} \\
&= \frac{c^{18}}{a^{12} b^{10}}
\end{aligned}$$

$$18. \left[\frac{p^{-6} q^7 (p^2 q)^{-3}}{(p^{-1} q^{-4})^2 p^{10}} \right]^3$$

$$\begin{aligned}
\left[\frac{p^{-6}q^7(p^2q)^{-3}}{(p^{-1}q^{-4})^2p^{10}} \right]^3 &= \left[\frac{p^{-6}q^7p^{2 \cdot (-3)}q^{-3}}{p^{-1 \cdot (2)}q^{-4 \cdot (2)}p^{10}} \right]^3 \\
&= \left[\frac{p^{-6}p^{-6}q^7q^{-3}}{p^{-2}p^{10}q^{-8}} \right]^3 \\
&= \left(\frac{p^{-6+(-6)}q^{7+(-3)}}{p^{-2+10}q^{-8}} \right)^3 \\
&= \left(\frac{p^{-12}q^4}{p^8q^{-8}} \right)^3 \\
&= (p^{-12-8}q^{4-(-8)})^3 \\
&= (p^{-20}q^{12})^3 \\
&= p^{-20 \cdot 3}q^{12 \cdot 3} \\
&= p^{-60}q^{36} \\
&= \frac{q^{36}}{p^{60}}
\end{aligned}$$

For problems 19 - 23, determine if the statement is true or false. If it is false, explain why it is false and give a corrected version of the statement.

19. $\frac{1}{6x} = 6x^{-1}$

The statement is false because given the property:

$$(ab)^{-n} = \frac{1}{(ab)^n} \text{ therefore}$$

$$6x^{-1} = \frac{6}{x} \quad \text{thus}$$

$$\frac{1}{6x} \neq \frac{6}{x}$$

A corrected version of the statement should look like this:

$$\frac{1}{6x} = (6x)^{-1}$$

20. $(x^3)^7 = x^{10}$

The statement is false because given the property:

$$(a^n)^m = a^{nm} \text{ therefore}$$

$$(x^3)^7 = x^{3 \cdot 7}$$

$$= x^{21} \text{ thus}$$

$$(x^3)^7 \neq x^{10}$$

A corrected version of the statement should look like this:

$$(x^3)^7 = x^{21}$$

$$21. (m^3n^4)^2 = m^{12}n^8$$

The statement is false because given the property:

$$(a^n b^m)^k = a^{nk} b^{mk}$$

Therefore, the corrected version of the statement should be:

$$(m^3n^4)^2 = m^6n^8$$

$$22. \left[(z^2)^3 \right]^4 = z^{24}$$

The statement is true.

$$23. (x + y)^3 = x^3 + y^3$$

The statement is false because expanding that expression gives us:

$$\begin{aligned} (x + y)^3 &= (x + y)(x + y)(x + y) \\ &= (x^2 + 2xy + y^2)(x + y) \\ &= x^3 + yx^2 + 2x^2y + 2xy^2 + yx^2 + y^3 \\ &= x^3 + 4x^2y + 2xy^2 + y^3 \end{aligned}$$

The corrected version of the statment is:

$$(x + y)^3 = x^3 + 4x^2y + 2xy^2 + y^3$$